<?xml version="1.0" encoding="UTF-8"?>

<rdf:RDF xmlns:rdf="http://www.w3.org/1999/02/22-rdf-syntax-ns#" xmlns:rdfs="http://www.w3.org/2000/01/rdf-schema#" xmlns:dc="http://purl.org/dc/elements/1.1/">

<rdf:Description rdf:about="http://www.w3.org/2003/01/geo/wgs84_pos#">
 <dc:title>WGS84 Geo Positioning: an RDF vocabulary</dc:title>
 <dc:description>A vocabulary for representing latitude, longitude and 
 altitude information in the WGS84 geodetic reference datum. 
 Version $Id: wgs84_pos.rdf,v 1.22 2009/04/20 15:00:30 timbl Exp $. See http://www.w3.org/2003/01/geo/ for more details.</dc:description>
 <dc:date>$Date: 2009/04/20 15:00:30 $</dc:date>
 <rdfs:label>geo</rdfs:label>
</rdf:Description>


<rdfs:Class rdf:about="http://www.w3.org/2003/01/geo/wgs84_pos#SpatialThing">
 <rdfs:label>SpatialThing</rdfs:label>
 <rdfs:comment>Anything with spatial extent, i.e. size, shape, or position.
 e.g. people, places, bowling balls, as well as abstract areas like cubes.
</rdfs:comment>
</rdfs:Class>

<!--
<rdfs:Class rdf:about="http://www.w3.org/2003/01/geo/wgs84_pos#TemporalThing">
 <rdfs:label>temporal thing</rdfs:label>
 <rdfs:comment>Anything with temporal extent, i.e. duration. e.g.
  the taking of a photograph, a scheduled meeting, a GPS timestamped trackpoint.
</rdfs:comment>
</rdfs:Class>

<rdfs:Class rdf:about="http://www.w3.org/2003/01/geo/wgs84_pos#Event">
  <rdfs:subClassOf rdf:resource="http://www.w3.org/2003/01/geo/wgs84_pos#TemporalThing" />
  <rdfs:label>event</rdfs:label>
  <rdfs:comment>An event, with negligible duration but unique date-time.
  Examples include a GPS timestamped trackpoint, the taking of a photograph,
  and the sending of a message.
  </rdfs:comment>
</rdfs:Class>
-->

<rdfs:Class rdf:about="http://www.w3.org/2003/01/geo/wgs84_pos#Point">
  <rdfs:subClassOf rdf:resource="http://www.w3.org/2003/01/geo/wgs84_pos#SpatialThing" />
  <rdfs:label>point</rdfs:label>
  <rdfs:comment>A point, typically described using a coordinate system relative to Earth, such as WGS84.
  </rdfs:comment>
  <rdfs:comment> 
Uniquely identified by lat/long/alt. i.e.

spaciallyIntersects(P1, P2) :- lat(P1, LAT), long(P1, LONG), alt(P1, ALT),
  lat(P2, LAT), long(P2, LONG), alt(P2, ALT).

sameThing(P1, P2) :- type(P1, Point), type(P2, Point), spaciallyIntersects(P1, P2).
  </rdfs:comment>
</rdfs:Class>


<rdf:Property rdf:about="http://www.w3.org/2003/01/geo/wgs84_pos#lat">
 <rdfs:domain rdf:resource="http://www.w3.org/2003/01/geo/wgs84_pos#SpatialThing" />
 <rdfs:label>latitude</rdfs:label>
 <rdfs:comment>The WGS84 latitude of a SpatialThing (decimal degrees).</rdfs:comment>
</rdf:Property>

<!--
<rdf:Property rdf:about="http://www.w3.org/2003/01/geo/wgs84_pos#time">
 <rdfs:domain rdf:resource="http://www.w3.org/2003/01/geo/wgs84_pos#TemporalThing" />
 <rdfs:label>time</rdfs:label>
 <rdfs:comment>The date time of an event, including fully qualified date,
    and Z or offset from UTC.  XML Schema standard
    date-time format.</rdfs:comment>
</rdf:Property>
-->

<rdf:Property rdf:about="http://www.w3.org/2003/01/geo/wgs84_pos#location">
 <rdfs:range rdf:resource="http://www.w3.org/2003/01/geo/wgs84_pos#SpatialThing" />
 <rdfs:label>location</rdfs:label>
 <rdfs:subPropertyOf rdf:resource="http://xmlns.com/foaf/0.1/based_near"/>
 <rdfs:comment>The relation between something and the point, 
 or other geometrical thing in space, where it is.  For example, the realtionship between
 a radio tower and a Point with a given lat and long.
 Or a relationship between a park and its outline as a closed arc of points, or a road and
 its location as a arc (a sequence of points).
 Clearly in practice there will be limit to the accuracy of any such statement, but one would expect
 an accuracy appropriate for the size of the object and uses such as mapping .
 </rdfs:comment>
</rdf:Property>

<rdf:Property rdf:about="http://www.w3.org/2003/01/geo/wgs84_pos#long">
 <rdfs:domain rdf:resource="http://www.w3.org/2003/01/geo/wgs84_pos#SpatialThing" />
 <rdfs:label>longitude</rdfs:label>
 <rdfs:comment>The WGS84 longitude of a SpatialThing (decimal degrees).</rdfs:comment>
</rdf:Property>

<rdf:Property rdf:about="http://www.w3.org/2003/01/geo/wgs84_pos#alt">
 <rdfs:domain rdf:resource="http://www.w3.org/2003/01/geo/wgs84_pos#SpatialThing" />
 <rdfs:label>altitude</rdfs:label>
 <rdfs:comment>The WGS84 altitude of a SpatialThing (decimal meters 
above the local reference ellipsoid).</rdfs:comment>
</rdf:Property>

<!-- not sure we really need this -->
<rdf:Property rdf:about="http://www.w3.org/2003/01/geo/wgs84_pos#lat_long">
 <rdfs:label>lat/long</rdfs:label>
 <rdfs:comment>A comma-separated representation of a latitude, longitude coordinate.</rdfs:comment>
</rdf:Property>

</rdf:RDF>
